Hoare/Hoare_Exp.thy
@@ -1,3 +1,6 @@
+(* Expressions as functions and relations, following chapter Imp in
+   "Software Foundations". *)
+
 theory Hoare_Exp
 imports "../Auto2"
 begin
@@ -7,8 +10,6 @@ datatype aexp =
 | APlus aexp aexp
 | AMinus aexp aexp
 | AMult aexp aexp
-
-thm aexp.induct
 
 datatype bexp =
   BTrue
@@ -43,13 +44,10 @@ inductive aevalR :: "aexp \<Rightarrow> nat \<Rightarrow> bool" (infix "\<Down>"
 | "e1 \<Down> n1 \<Longrightarrow> e2 \<Down> n2 \<Longrightarrow> (APlus e1 e2) \<Down> (n1 + n2)"
 | "e1 \<Down> n1 \<Longrightarrow> e2 \<Down> n2 \<Longrightarrow> (AMinus e1 e2) \<Down> (n1 - n2)"
 | "e1 \<Down> n1 \<Longrightarrow> e2 \<Down> n2 \<Longrightarrow> (AMult e1 e2) \<Down> (n1 * n2)"
-setup {* add_known_fact @{thm aevalR.intros(1)} *}
+setup {* add_resolve_prfstep @{thm aevalR.intros(1)} *}
 setup {* fold add_backward2_prfstep
   [@{thm aevalR.intros(2)}, @{thm aevalR.intros(3)}, @{thm aevalR.intros(4)}] *}
 setup {* add_prfstep_prop_induction @{thm aevalR.induct} *}
-
-theorem test_aevalR1: "(APlus (ANum 2) (ANum 2)) \<Down> 4"
-  by (metis aeval.simps(1) aeval.simps(2) aevalR.intros(1) aevalR.intros(2) test_aeval1)
 
 inductive bevalR :: "bexp \<Rightarrow> bool \<Rightarrow> bool" where
   "bevalR BTrue True"
@@ -60,29 +58,27 @@ inductive bevalR :: "bexp \<Rightarrow> bool \<Rightarrow> bool" where
 | "bevalR b1 v1 \<Longrightarrow> bevalR b2 v2 \<Longrightarrow> bevalR (BAnd b1 b2) (v1 \<and> v2)"
 theorem bevalR_intros1': "v \<Longrightarrow> bevalR BTrue v" by (simp add: bevalR.intros(1))
 theorem bevalR_intros2': "\<not>v \<Longrightarrow> bevalR BFalse v" by (simp add: bevalR.intros(2))
-setup {* add_prfstep_prop_induction @{thm bevalR.induct} *}
 setup {* fold add_backward_prfstep [@{thm bevalR_intros1'}, @{thm bevalR_intros2'}, @{thm bevalR.intros(5)}] *}
 setup {* fold add_backward2_prfstep [@{thm bevalR.intros(3)}, @{thm bevalR.intros(4)}, @{thm bevalR.intros(6)}] *}
-
-theorem test_bevalR1: "bevalR (BEq (ANum 2) (ANum 3)) False"
-  by (metis (full_types) aevalR.intros(1) bevalR.intros(3) numeral_eq_iff semiring_norm(88))
+setup {* add_prfstep_prop_induction @{thm bevalR.induct} *}
 
 setup {* add_prfstep_var_induction @{thm aexp.induct} *}
 setup {* add_prfstep_var_induction @{thm bexp.induct} *}
 
 (* Equivalence of definitions. *)
-theorem aevalR_to_aeval [forward]: "a \<Down> n \<Longrightarrow> aeval a = n" by auto2
-theorem aeval_to_aevalR: "aeval a = n \<Longrightarrow> a \<Down> n"
-  by (tactic {* auto2s_tac @{context} (VAR_INDUCT ("a", [Arbitrary "n"])) *})
-theorem aeval_to_aevalR': "a \<Down> aeval a" by (simp add: aeval_to_aevalR)
-setup {* add_forward_prfstep_cond @{thm aeval_to_aevalR'} [with_term "aeval ?a"] *}
-theorem aeval_iff_aevalR: "a \<Down> n \<longleftrightarrow> aeval a = n" by auto2
+theorem aeval_iff_aevalR [rewrite]: "a \<Down> n \<longleftrightarrow> aeval a = n"
+  by (tactic {* auto2s_tac @{context}
+    (OBTAIN "\<forall>a' n'. a' \<Down> n' \<longrightarrow> aeval a' = n'" WITH PROP_INDUCT ("a' \<Down> n'", []) THEN
+     OBTAIN "\<forall>a' n'. aeval a' = n' \<longrightarrow> a' \<Down> n'" WITH VAR_INDUCT ("a'", [Arbitrary "n'"])) *})
+theorem aevalR_triv: "a \<Down> aeval a" by auto2
+setup {* add_forward_prfstep_cond @{thm aevalR_triv} [with_term "aeval ?a"] *}
+theorem test_aevalR1: "(APlus (ANum 2) (ANum 2)) \<Down> 4" by auto2
 
-theorem bevalR_to_beval [forward]: "bevalR b v \<Longrightarrow> (beval b = v)" by auto2
-theorem beval_to_bevalR: "(beval b = v) \<Longrightarrow> bevalR b v"
-  by (tactic {* auto2s_tac @{context} (VAR_INDUCT ("b", [Arbitrary "v"])) *})
-theorem beval_to_bevalR': "bevalR b (beval b)" by (simp add: beval_to_bevalR)
-setup {* add_forward_prfstep_cond @{thm beval_to_bevalR'} [with_term "beval ?b"] *}
-theorem beval_iff_bevalR: "bevalR b v \<longleftrightarrow> (beval b = v)" by auto2
+theorem beval_iff_bevalR [rewrite]: "bevalR b v \<longleftrightarrow> beval b = v"
+  by (tactic {* auto2s_tac @{context}
+    (OBTAIN "\<forall>b' v'. bevalR b' v' \<longrightarrow> beval b' = v'" WITH PROP_INDUCT ("bevalR b' v'", []) THEN
+     OBTAIN "\<forall>b' v'. beval b' = v' \<longrightarrow> bevalR b' v'" WITH VAR_INDUCT ("b'", [Arbitrary "v'"])) *})
+theorem bevalR_triv: "bevalR b (beval b)" by auto2
+theorem test_bevalR1: "bevalR (BEq (ANum 2) (ANum 3)) False" by auto2
 
 end
