Auto2_Base.thy
@@ -1,3 +1,5 @@
+(* Auto2 tactic. *)
+
 theory Auto2_Base
 imports Main Logic_Base
 begin
@@ -16,14 +18,6 @@ ML_file "induction.ML"
 
 method_setup auto2 = {* Scan.succeed (SIMPLE_METHOD o auto2_tac) *} "auto2 prover"
 
-text {* First add proofstep converting any PROP equality to EQ. Then use EQ to match
-  equality in all proofsteps. *}
-theorem trivial_eq: "A = B \<Longrightarrow> A = B" by simp
-setup {* add_gen_prfstep ("trivial_eq",
-  [WithItem (TY_PROP, @{term_pat "(?A::?'a) = ?B"}),
-   GetFact (@{term_pat "(?A::?'a) = ?B"}, @{thm trivial_eq})]) *}
-
-attribute_setup known_fact = {* setup_attrib add_known_fact_ctxt *}
 attribute_setup forward = {* setup_attrib add_forward_prfstep_ctxt *}
 attribute_setup backward = {* setup_attrib add_backward_prfstep_ctxt *}
 attribute_setup backward1 = {* setup_attrib add_backward1_prfstep_ctxt *}
