Logic_Thms.thy
@@ -1,6 +1,15 @@
+(* Setup for proof steps related to logic. *)
+
 theory Logic_Thms
 imports Auto2_Base
 begin
+
+(* First add proofstep converting any PROP equality to EQ. Then use EQ to match
+   equality in all proofsteps. *)
+theorem trivial_eq: "A = B \<Longrightarrow> A = B" by simp
+setup {* add_gen_prfstep ("trivial_eq",
+  [WithItem (TY_PROP, @{term_pat "(?A::?'a) = ?B"}),
+   GetFact (@{term_pat "(?A::?'a) = ?B"}, @{thm trivial_eq})]) *}
 
 setup {* fold add_rew_const [@{term "True"}, @{term "False"}] *}
 setup {* fold add_th_normalizer
@@ -31,7 +40,7 @@ ML {*
 (* Rewrites A = True to A, etc. *)
 theorem neq_True: "(A \<noteq> True) = (\<not>A)" by simp
 theorem neq_False: "(A \<noteq> False) = A" by simp
-setup {* fold add_eq_th_normalizer
+setup {* fold (fn th => add_eq_th_normalizer th #> add_top_eq_th_normalizer th)
   [@{thm HOL.eq_True}, @{thm HOL.eq_False}, @{thm neq_True}, @{thm neq_False}] *}
 
 (* Trivial contradictions. *)
@@ -54,49 +63,60 @@ setup {* add_forward_prfstep_cond @{thm HOL.not_sym} [with_filt (not_type_filter
 
 (* Iff. *)
 setup {* add_gen_prfstep ("iff_intro1",
-  [WithGoal @{term_pat "(?A::bool) = ?B"},
-   CreateCase ([@{term_pat "?A::bool"}], [@{term_pat "?B::bool"}])]) *}
+  [WithGoal @{term_pat "(?A::bool) = ?B"}, CreateCase @{term_pat "?A::bool"}]) *}
 setup {* add_fixed_sc ("iff_intro1", 25) *}  (* includes the cost of creating a case. *)
-theorem iff_intro2 [forward]: "A \<longrightarrow> B \<Longrightarrow> \<not>(A \<longleftrightarrow> B) \<Longrightarrow> \<not>A \<and> B" by simp
-setup {* add_fixed_sc ("Logic_Thms.iff_intro2", 1) *}
+theorem iff_two_dirs [forward]: "A \<noteq> B \<Longrightarrow> (A \<longrightarrow> \<not>B) \<and> (\<not>A \<longrightarrow> B)" by auto
+setup {* add_fixed_sc ("Logic_Thms.iff_two_dirs", 1) *}
 
 (* Implies. *)
 setup {* add_forward_prfstep @{thm Meson.not_impD} *}
 setup {* add_fixed_sc ("Meson.not_impD", 1) *}
 lemma not_conj_to_imp: "\<not>(A \<and> B) \<longleftrightarrow> A \<longrightarrow> \<not>B" by simp  (* used in not_ex_forall_cv *)
 
-(* Quantifiers: splitting. *)
-setup {* add_forward_prfstep (equiv_forward_th @{thm all_conj_distrib}) *}
+(* Quantifiers: normalization *)
 theorem forall_or [forward]:
   "(\<forall>x. ((A x \<or> B x) \<longrightarrow> C x)) \<Longrightarrow> ((\<forall>x. A x \<longrightarrow> C x) \<and> (\<forall>x. B x \<longrightarrow> C x))" by blast
+
+theorem contract_not_forall: "\<not>(\<forall>x. P) \<longleftrightarrow> \<not>P" by simp
+ML {*
+val forall_norm_ths = [
+  @{thm all_conj_distrib}, @{thm use_vardef}, @{thm HOL.all_simps(6)},
+  @{thm HOL.simp_thms(35)}, @{thm contract_not_forall}]
+*}
+setup {* fold add_eq_th_normalizer forall_norm_ths *}
+setup {* add_backward_prfstep (equiv_backward_th @{thm ex_disj_distrib}) *}
 theorem exists_split: "(\<exists>x y. P x \<and> Q y) = ((\<exists>x. P x) \<and> (\<exists>y. Q y))" by simp
 setup {* add_backward_prfstep (equiv_backward_th @{thm exists_split}) *}
-setup {* add_backward_prfstep (equiv_backward_th @{thm ex_disj_distrib}) *}
 
-(* Quantifiers: swapping out of ALL or EX *)
-theorem swap_forall_imp: "(\<forall>x. P \<longrightarrow> Q x) \<longleftrightarrow> (P \<longrightarrow> (\<forall>x. Q x))" by auto
-theorem swap_ex_conj: "(\<exists>x. P \<and> Q x) \<longleftrightarrow> (P \<and> (\<exists>x. Q x))" by auto
-
-(* (\<forall>x. x = ?t \<longrightarrow> ?P x) = ?P ?t *)
-setup {* add_eq_th_normalizer @{thm use_vardef} *}
-(* (\<forall>x. ?P \<longrightarrow> ?Q x) = (?P \<longrightarrow> (\<forall>x. ?Q x)) *)
-setup {* add_eq_th_normalizer @{thm HOL.all_simps(6)} *}
+(* Bounded quantifiers. *)
+setup {* add_backward_prfstep (equiv_backward_th @{thm bex_iff}) *}
 
 (* Case analysis. *)
 setup {* add_gen_prfstep ("case_intro",
   [WithTerm @{term_pat "if ?cond then (?yes::?'a) else ?no"},
-   CreateCase ([@{term_pat "?cond::bool"}], [])]) *}
-theorem if_eq: "(if a = a then x else y) = x" by simp
+   CreateCase @{term_pat "?cond::bool"}]) *}
 theorem if_not_P': "P \<Longrightarrow> (if \<not>P then x else y) = y" by simp
 setup {* fold add_rewrite_rule [@{thm HOL.if_P}, @{thm HOL.if_not_P}, @{thm if_not_P'}] *}
 setup {* fold add_fixed_sc [("HOL.if_P", 1), ("HOL.if_not_P", 1), ("Logic_Thms.if_not_P'", 1)] *}
 
 (* Hilbert choice. *)
 setup {* add_gen_prfstep ("SOME_case_intro",
-  [WithTerm @{term_pat "SOME k. ?P k"},
-   CreateCase ([], [@{term_pat "\<exists>k. ?P k"}])]) *}
+  [WithTerm @{term_pat "SOME k. ?P k"}, CreateConcl @{term_pat "\<exists>k. ?P k"}]) *}
 setup {* add_forward_prfstep_cond @{thm someI} [with_term "SOME x. ?P x"] *}
 setup {* add_forward_prfstep_cond @{thm someI_ex} [with_term "SOME x. ?P x"] *}
+
+(* Axiom of choice *)
+setup {* add_prfstep_custom ("ex_choice",
+  [WithGoal @{term_pat "EX f. !x. ?Q f x"}],
+  [Update.ADD_ITEMS],
+  (fn ((id, _), ths) => fn _ => fn _ =>
+    [Update.thm_update (id, (ths MRS (backward_th @{thm choice})))]
+    handle THM _ => []))
+*}
+
+(* Extensionality. *)
+theorem set_ext [resolve]: "\<forall>a. a \<in> S \<longleftrightarrow> a \<in> T \<Longrightarrow> S = T" by auto
+theorem set_pair_ext [resolve]: "\<forall>a b. (a, b) \<in> S \<longleftrightarrow> (a, b) \<in> T \<Longrightarrow> S = T" by auto
 
 (* Least operator. *)
 theorem Least_equality' [backward1]:
@@ -108,6 +128,13 @@ setup {* add_rewrite_rule @{thm snd_conv} *}
 
 (* Let. *)
 setup {* add_rewrite_rule (to_obj_eq_th @{thm Let_def}) *}
+
+(* Eta contraction *)
+setup {* add_prfstep_conv ("eta_contract", [WithTerm @{term_pat "?A"}], Thm.eta_conversion) *}
+
+(* Equivalence relation *)
+setup {* add_rewrite_rule @{thm symp_def} *}
+setup {* add_rewrite_rule @{thm transp_def} *}
 
 (* Quantifiers and other fundamental proofsteps. *)
 ML_file "logic_steps.ML"
